Parikh/Lfun.thy
@@ -19,16 +19,16 @@ datatype 'a lfun = Var nat                        (* Variable *)
                  | Star "'a lfun"
 
 (* instantiate each variable with a language *)
-type_synonym 'a state = "nat \<Rightarrow> 'a lang"
+type_synonym 'a valuation = "nat \<Rightarrow> 'a lang"
 
 (* evaluate function for a given state, this produces a language *)
-primrec eval :: "'a lfun \<Rightarrow> 'a state \<Rightarrow> 'a lang" where
-  "eval (Var n) s = s n" |
+primrec eval :: "'a lfun \<Rightarrow> 'a valuation \<Rightarrow> 'a lang" where
+  "eval (Var n) v = v n" |
   "eval (Const l) _ = l" |
-  "eval (Union2 f g) s = eval f s \<union> eval g s" |
-  "eval (UnionC f) s = (\<Union>i. eval (f i) s)" |
-  "eval (Concat f g) s = eval f s @@ eval g s" |
-  "eval (Star f) s = star (eval f s)"
+  "eval (Union2 f g) v = eval f v \<union> eval g v" |
+  "eval (UnionC f) v = (\<Union>i. eval (f i) v)" |
+  "eval (Concat f g) v = eval f v @@ eval g v" |
+  "eval (Star f) v = star (eval f v)"
 
 (* all variables occurring in a function *)
 primrec vars :: "'a lfun \<Rightarrow> nat set" where
@@ -40,55 +40,55 @@ primrec vars :: "'a lfun \<Rightarrow> nat set" where
   "vars (Star f) = vars f"
 
 (* substitute each occurrence of a variable i by the language function s i *)
-primrec subst :: "'a lfun \<Rightarrow> (nat \<Rightarrow> 'a lfun) \<Rightarrow> 'a lfun" where
-  "subst (Var n) s = s n" |
-  "subst (Const l) _ = Const l" |
-  "subst (Union2 f g) s = Union2 (subst f s) (subst g s)" |
-  "subst (UnionC f) s = UnionC (\<lambda>i. subst (f i) s)" |
-  "subst (Concat f g) s = Concat (subst f s) (subst g s)" |
-  "subst (Star f) s = Star (subst f s)"
+primrec subst :: "(nat \<Rightarrow> 'a lfun) \<Rightarrow> 'a lfun \<Rightarrow> 'a lfun" where
+  "subst s (Var n) = s n" |
+  "subst _ (Const l) = Const l" |
+  "subst s (Union2 f g) = Union2 (subst s f) (subst s g)" |
+  "subst s (UnionC f) = UnionC (\<lambda>i. subst s (f i))" |
+  "subst s (Concat f g) = Concat (subst s f) (subst s g)" |
+  "subst s (Star f) = Star (subst s f)"
 
 
 
 section \<open>Some lemmas about the introduced functions\<close>
 
 lemma substitution_lemma:
-  assumes "\<forall>i. s' i = eval (upd i) s"
-  shows "eval (subst f upd) s = eval f s'"
+  assumes "\<forall>i. v' i = eval (upd i) v"
+  shows "eval (subst upd f) v = eval f v'"
   using assms by (induction rule: lfun.induct) auto
 
 lemma substitution_lemma_update:
-  "eval (subst f (Var(x := f'))) s = eval f (s(x := eval f' s))"
-  using substitution_lemma[of "s(x := eval f' s)"] by force
+  "eval (subst (Var(x := f')) f) v = eval f (v(x := eval f' v))"
+  using substitution_lemma[of "v(x := eval f' v)"] by force
 
-lemma subst_id: "eval (subst f Var) s = eval f s"
-  using substitution_lemma[of s] by simp
+lemma subst_id: "eval (subst Var f) v = eval f v"
+  using substitution_lemma[of v] by simp
 
 
-lemma vars_subst: "vars (subst f upd) = (\<Union>x \<in> vars f. vars (upd x))"
+lemma vars_subst: "vars (subst upd f) = (\<Union>x \<in> vars f. vars (upd x))"
   by (induction f) auto
 
-lemma vars_subst_upper: "vars (subst f upd) \<subseteq> (\<Union>x. vars (upd x))"
+lemma vars_subst_upper: "vars (subst upd f) \<subseteq> (\<Union>x. vars (upd x))"
   using vars_subst by force
 
 
-lemma vars_subst_upd_upper: "vars (subst f (Var(x := fx))) \<subseteq> vars f - {x} \<union> vars fx"
+lemma vars_subst_upd_upper: "vars (subst (Var(x := fx)) f) \<subseteq> vars f - {x} \<union> vars fx"
 proof
   fix y
   let ?upd = "Var(x := fx)"
-  assume "y \<in> vars (subst f ?upd)"
+  assume "y \<in> vars (subst ?upd f)"
   then obtain y' where "y' \<in> vars f \<and> y \<in> vars (?upd y')" using vars_subst by blast
   then show "y \<in> vars f - {x} \<union> vars fx" by (cases "x = y'") auto
 qed
 
 lemma vars_subst_upd_aux:
   assumes "x \<in> vars f"
-  shows   "vars f - {x} \<union> vars fx \<subseteq> vars (subst f (Var(x := fx)))"
+  shows   "vars f - {x} \<union> vars fx \<subseteq> vars (subst (Var(x := fx)) f)"
 proof
   fix y
   let ?upd = "Var(x := fx)"
   assume as: "y \<in> vars f - {x} \<union> vars fx"
-  then show "y \<in> vars (subst f ?upd)"
+  then show "y \<in> vars (subst ?upd f)"
   proof (cases "y \<in> vars f - {x}")
     case True
     then show ?thesis using vars_subst by fastforce
@@ -101,7 +101,7 @@ qed
 
 lemma vars_subst_upd:
   assumes "x \<in> vars f"
-  shows   "vars (subst f (Var(x := fx))) = vars f - {x} \<union> vars fx"
+  shows   "vars (subst (Var(x := fx)) f) = vars f - {x} \<union> vars fx"
   using assms vars_subst_upd_upper vars_subst_upd_aux by blast
 
 lemma eval_vars:
@@ -110,17 +110,17 @@ lemma eval_vars:
   using assms by (induction f) auto
 
 lemma eval_vars_subst:
-  assumes "\<forall>i \<in> vars f. s i = eval (upd i) s"
-  shows "eval (subst f upd) s = eval f s"
+  assumes "\<forall>i \<in> vars f. v i = eval (upd i) v"
+  shows "eval (subst upd f) v = eval f v"
 proof -
-  let ?s' = "\<lambda>i. if i \<in> vars f then s i else eval (upd i) s"
-  let ?s'' = "\<lambda>i. eval (upd i) s"
-  have s'_s'': "?s' i = ?s'' i" for i using assms by simp
-  then have s_s'': "\<forall>i. ?s'' i = eval (upd i) s" by simp
+  let ?v' = "\<lambda>i. if i \<in> vars f then v i else eval (upd i) v"
+  let ?v'' = "\<lambda>i. eval (upd i) v"
+  have v'_v'': "?v' i = ?v'' i" for i using assms by simp
+  then have v_v'': "\<forall>i. ?v'' i = eval (upd i) v" by simp
 
-  from assms have "eval f s = eval f ?s'" using eval_vars[of f] by simp
-  also have "\<dots> = eval (subst f upd) s"
-    using assms substitution_lemma[OF s_s'', of f] by (simp add: eval_vars)
+  from assms have "eval f v = eval f ?v'" using eval_vars[of f] by simp
+  also have "\<dots> = eval (subst upd f) v"
+    using assms substitution_lemma[OF v_v'', of f] by (simp add: eval_vars)
   finally show ?thesis by simp
 qed
 
@@ -129,8 +129,8 @@ qed
 section \<open>Monotonicity of language functions\<close>
 
 lemma lfun_mono_aux:
-  assumes "\<forall>i \<in> vars f. s i \<subseteq> s' i"
-  shows "eval f s \<subseteq> eval f s'"
+  assumes "\<forall>i \<in> vars f. v i \<subseteq> v' i"
+  shows "eval f v \<subseteq> eval f v'"
 using assms proof (induction rule: lfun.induct)
   case (Star x)
   then show ?case
@@ -154,71 +154,71 @@ lemma langpow_mono:
 using assms conc_mono[of A B] by (induction n) auto
 
 lemma lfun_cont_aux1:
-  assumes "\<forall>i. s i \<le> s (Suc i)"
-      and "w \<in> (\<Union>i. eval f (s i))"
-    shows "w \<in> eval f (\<lambda>x. \<Union>i. s i x)"
+  assumes "\<forall>i. v i \<le> v (Suc i)"
+      and "w \<in> (\<Union>i. eval f (v i))"
+    shows "w \<in> eval f (\<lambda>x. \<Union>i. v i x)"
 proof -
-  from assms(2) obtain n where n_intro: "w \<in> eval f (s n)" by auto
-  have "s n x \<subseteq> (\<Union>i. s i x)" for x by auto
+  from assms(2) obtain n where n_intro: "w \<in> eval f (v n)" by auto
+  have "v n x \<subseteq> (\<Union>i. v i x)" for x by auto
   with n_intro show "?thesis"
-    using lfun_mono_aux[where s="s n" and s'="\<lambda>x. \<Union>i. s i x"] by auto
+    using lfun_mono_aux[where v="v n" and v'="\<lambda>x. \<Union>i. v i x"] by auto
 qed
 
 lemma langpow_Union_eval:
-  assumes "\<forall>i. s i \<le> s (Suc i)"
-      and "w \<in> (\<Union>i. eval f (s i)) ^^ n"
-    shows "w \<in> (\<Union>i. eval f (s i) ^^ n)"
+  assumes "\<forall>i. v i \<le> v (Suc i)"
+      and "w \<in> (\<Union>i. eval f (v i)) ^^ n"
+    shows "w \<in> (\<Union>i. eval f (v i) ^^ n)"
 using assms proof (induction n arbitrary: w)
   case 0
   then show ?case by simp
 next
   case (Suc n)
-  then obtain u v where w_decomp: "w = u@v" and
-    "u \<in> (\<Union>i. eval f (s i)) \<and> v \<in> (\<Union>i. eval f (s i)) ^^ n" by fastforce
-  with Suc have "u \<in> (\<Union>i. eval f (s i)) \<and> v \<in> (\<Union>i. eval f (s i) ^^ n)" by auto
-  then obtain i j where i_intro: "u \<in> eval f (s i)" and j_intro: "v \<in> eval f (s j) ^^ n" by blast
+  then obtain u u' where w_decomp: "w = u@u'" and
+    "u \<in> (\<Union>i. eval f (v i)) \<and> u' \<in> (\<Union>i. eval f (v i)) ^^ n" by fastforce
+  with Suc have "u \<in> (\<Union>i. eval f (v i)) \<and> u' \<in> (\<Union>i. eval f (v i) ^^ n)" by auto
+  then obtain i j where i_intro: "u \<in> eval f (v i)" and j_intro: "u' \<in> eval f (v j) ^^ n" by blast
   let ?m = "max i j"
-  from i_intro Suc.prems(1) lfun_mono_aux have 1: "u \<in> eval f (s ?m)"
+  from i_intro Suc.prems(1) lfun_mono_aux have 1: "u \<in> eval f (v ?m)"
     by (metis le_fun_def lift_Suc_mono_le max.cobounded1 subset_eq)
-  from Suc.prems(1) lfun_mono_aux have "eval f (s j) \<subseteq> eval f (s ?m)"
+  from Suc.prems(1) lfun_mono_aux have "eval f (v j) \<subseteq> eval f (v ?m)"
     by (metis le_fun_def lift_Suc_mono_le max.cobounded2)
-  with j_intro langpow_mono have 2: "v \<in> eval f (s ?m) ^^ n" by auto
+  with j_intro langpow_mono have 2: "u' \<in> eval f (v ?m) ^^ n" by auto
   from 1 2 show ?case using w_decomp by auto
 qed
 
 lemma lfun_cont_aux2:
-  assumes "\<forall>i. s i \<le> s (Suc i)"
-      and "w \<in> eval f (\<lambda>x. \<Union>i. s i x)"
-    shows "w \<in> (\<Union>i. eval f (s i))"
+  assumes "\<forall>i. v i \<le> v (Suc i)"
+      and "w \<in> eval f (\<lambda>x. \<Union>i. v i x)"
+    shows "w \<in> (\<Union>i. eval f (v i))"
 using assms proof (induction arbitrary: w rule: lfun.induct)
   case (Concat f g)
-  then obtain u v where w_decomp: "w = u@v"
-    and "u \<in> eval f (\<lambda>x. \<Union>i. s i x) \<and> v \<in> eval g (\<lambda>x. \<Union>i. s i x)" by auto
-  with Concat have "u \<in> (\<Union>i. eval f (s i)) \<and> v \<in> (\<Union>i. eval g (s i))" by auto
-  then obtain i j where i_intro: "u \<in> eval f (s i)" and j_intro: "v \<in> eval g (s j)" by blast
+  then obtain u u' where w_decomp: "w = u@u'"
+    and "u \<in> eval f (\<lambda>x. \<Union>i. v i x) \<and> u' \<in> eval g (\<lambda>x. \<Union>i. v i x)" by auto
+  with Concat have "u \<in> (\<Union>i. eval f (v i)) \<and> u' \<in> (\<Union>i. eval g (v i))" by auto
+  then obtain i j where i_intro: "u \<in> eval f (v i)" and j_intro: "u' \<in> eval g (v j)" by blast
   let ?m = "max i j"
-  from i_intro Concat.prems(1) lfun_mono_aux have "u \<in> eval f (s ?m)"
+  from i_intro Concat.prems(1) lfun_mono_aux have "u \<in> eval f (v ?m)"
     by (metis le_fun_def lift_Suc_mono_le max.cobounded1 subset_eq)
-  moreover from j_intro Concat.prems(1) lfun_mono_aux have "v \<in> eval g (s ?m)"
+  moreover from j_intro Concat.prems(1) lfun_mono_aux have "u' \<in> eval g (v ?m)"
     by (metis le_fun_def lift_Suc_mono_le max.cobounded2 subset_eq)
   ultimately show ?case using w_decomp by auto
 next
   case (Star f)
-  then obtain n where n_intro: "w \<in> (eval f (\<lambda>x. \<Union>i. s i x)) ^^ n"
+  then obtain n where n_intro: "w \<in> (eval f (\<lambda>x. \<Union>i. v i x)) ^^ n"
     using eval.simps(6) star_pow by blast
-  with Star have "w \<in> (\<Union>i. eval f (s i)) ^^ n" using langpow_mono by blast
-  with Star.prems have "w \<in> (\<Union>i. eval f (s i) ^^ n)" using langpow_Union_eval by auto
+  with Star have "w \<in> (\<Union>i. eval f (v i)) ^^ n" using langpow_mono by blast
+  with Star.prems have "w \<in> (\<Union>i. eval f (v i) ^^ n)" using langpow_Union_eval by auto
   then show ?case by (auto simp add: star_def)
 qed fastforce+
 
 
 (* The actual continuity lemma *)
 lemma lfun_cont:
-  assumes "\<forall>i. s i \<le> s (Suc i)"
-  shows "eval f (\<lambda>x. \<Union>i. s i x) = (\<Union>i. eval f (s i))"
+  assumes "\<forall>i. v i \<le> v (Suc i)"
+  shows "eval f (\<lambda>x. \<Union>i. v i x) = (\<Union>i. eval f (v i))"
 proof
-  from assms show "eval f (\<lambda>x. \<Union>i. s i x) \<subseteq> (\<Union>i. eval f (s i))" using lfun_cont_aux2 by auto
-  from assms show "(\<Union>i. eval f (s i)) \<subseteq> eval f (\<lambda>x. \<Union>i. s i x)" using lfun_cont_aux1 by blast
+  from assms show "eval f (\<lambda>x. \<Union>i. v i x) \<subseteq> (\<Union>i. eval f (v i))" using lfun_cont_aux2 by auto
+  from assms show "(\<Union>i. eval f (v i)) \<subseteq> eval f (\<lambda>x. \<Union>i. v i x)" using lfun_cont_aux1 by blast
 qed
 
 
@@ -255,22 +255,22 @@ lemma epsilon_regular: "regular_fun (Const {[]})"
 (* If all arguments are regular, a regular function evaluates to a regular language *)
 lemma regular_fun_regular:
   assumes "regular_fun f"
-      and "\<And>n. n \<in> vars f \<Longrightarrow> regular_lang (s n)"
-    shows "regular_lang (eval f s)"
+      and "\<And>n. n \<in> vars f \<Longrightarrow> regular_lang (v n)"
+    shows "regular_lang (eval f v)"
 using assms proof (induction rule: regular_fun.induct)
   case (Union2 f g)
-  then obtain r1 r2 where "Regular_Exp.lang r1 = eval f s \<and> Regular_Exp.lang r2 = eval g s" by auto
-  then have "Regular_Exp.lang (Plus r1 r2) = eval (Union2 f g) s" by simp
+  then obtain r1 r2 where "Regular_Exp.lang r1 = eval f v \<and> Regular_Exp.lang r2 = eval g v" by auto
+  then have "Regular_Exp.lang (Plus r1 r2) = eval (Union2 f g) v" by simp
   then show ?case by blast
 next
   case (Concat f g)
-  then obtain r1 r2 where "Regular_Exp.lang r1 = eval f s \<and> Regular_Exp.lang r2 = eval g s" by auto
-  then have "Regular_Exp.lang (Times r1 r2) = eval (Concat f g) s" by simp
+  then obtain r1 r2 where "Regular_Exp.lang r1 = eval f v \<and> Regular_Exp.lang r2 = eval g v" by auto
+  then have "Regular_Exp.lang (Times r1 r2) = eval (Concat f g) v" by simp
   then show ?case by blast
 next
   case (Star f)
-  then obtain r  where "Regular_Exp.lang r = eval f s" by auto
-  then have "Regular_Exp.lang (Regular_Exp.Star r) = eval (Star f) s" by simp
+  then obtain r  where "Regular_Exp.lang r = eval f v" by auto
+  then have "Regular_Exp.lang (Regular_Exp.Star r) = eval (Star f) v" by simp
   then show ?case by blast
 qed auto
 
@@ -279,27 +279,27 @@ qed auto
 lemma subst_reg_fun:
   assumes "regular_fun f"
       and "\<forall>x \<in> vars f. regular_fun (upd x)"
-    shows "regular_fun (subst f upd)"
+    shows "regular_fun (subst upd f)"
   using assms by (induction rule: regular_fun.induct) auto
 
 
 lemma subst_reg_fun_update:
   assumes "regular_fun f"
       and "regular_fun g"
-    shows "regular_fun (subst f (Var(x := g)))"
+    shows "regular_fun (subst (Var(x := g)) f)"
   using assms subst_reg_fun fun_upd_def by (metis Variable)
 
 
 lemma finite_Union_regular_aux:
   "\<forall>f \<in> set fs. regular_fun f \<Longrightarrow> \<exists>g. regular_fun g \<and> \<Union>(vars ` set fs) = vars g
-                                      \<and> (\<forall>s. (\<Union>f \<in> set fs. eval f s) = eval g s)"
+                                      \<and> (\<forall>v. (\<Union>f \<in> set fs. eval f v) = eval g v)"
 proof (induction fs)
   case Nil
   then show ?case using emptyset_regular by force
 next
   case (Cons f1 fs)
   then obtain g where *: "regular_fun g \<and> \<Union>(vars ` set fs) = vars g
-                          \<and> (\<forall>s. (\<Union>f\<in>set fs. eval f s) = eval g s)" by auto
+                          \<and> (\<forall>v. (\<Union>f\<in>set fs. eval f v) = eval g v)" by auto
   let ?g' = "Union2 f1 g"
   from Cons.prems * show ?case by auto
 qed
@@ -308,7 +308,7 @@ qed
 lemma finite_Union_regular:
   assumes "finite F"
       and "\<forall>f \<in> F. regular_fun f"
-    shows "\<exists>g. regular_fun g \<and> \<Union>(vars ` F) = vars g \<and> (\<forall>s. (\<Union>f\<in>F. eval f s) = eval g s)"
+    shows "\<exists>g. regular_fun g \<and> \<Union>(vars ` F) = vars g \<and> (\<forall>v. (\<Union>f\<in>F. eval f v) = eval g v)"
   using assms finite_Union_regular_aux finite_list by metis
 
 
@@ -318,7 +318,7 @@ section \<open>Constant functions\<close>
 abbreviation const_fun :: "'a lfun \<Rightarrow> bool" where
   "const_fun f \<equiv> vars f = {}"
 
-lemma const_fun_lang: "const_fun f \<Longrightarrow> \<exists>l. \<forall>s. eval f s = l"
+lemma const_fun_lang: "const_fun f \<Longrightarrow> \<exists>l. \<forall>v. eval f v = l"
 proof (induction f)
   case (UnionC x)
   then show ?case by (metis emptyE eval_vars)
@@ -327,7 +327,7 @@ qed auto
 lemma const_fun_regular_lang:
   assumes "const_fun f"
       and "regular_fun f"
-    shows "\<exists>l. regular_lang l \<and> (\<forall>s. eval f s = l)"
+    shows "\<exists>l. regular_lang l \<and> (\<forall>v. eval f v = l)"
   using assms const_fun_lang regular_fun_regular by fastforce
 
 end
