Parikh/Pilling.thy
@@ -28,13 +28,13 @@ lemma "regular_fun' x f \<Longrightarrow> regular_fun f"
 text \<open>Every regular function can be represented as regular_fun':\<close>
 
 lemma regular_fun_regular_fun'_Variable: "\<exists>f'. regular_fun' x f' \<and> vars f' = vars (Var y) \<union> {x}
-                                        \<and> (\<forall>s. parikh_img (eval (Var y) s) = parikh_img (eval f' s))"
+                                        \<and> (\<forall>v. parikh_img (eval (Var y) v) = parikh_img (eval f' v))"
 proof (cases "x = y")
 let ?f' = "Union2 (Const {}) (Concat (Const {[]}) (Var x))"
   case True
   then have "regular_fun' x ?f'"
     unfolding regular_fun'_def by (simp add: emptyset_regular epsilon_regular)
-  moreover have "eval ?f' s = eval (Var y) s" for s :: "'a state" using True by simp
+  moreover have "eval ?f' v = eval (Var y) v" for v :: "'a valuation" using True by simp
   moreover have "vars ?f' = vars (Var y) \<union> {x}" using True by simp
   ultimately show ?thesis by metis
 next
@@ -42,7 +42,7 @@ next
   case False
   then have "regular_fun' x ?f'"
     unfolding regular_fun'_def by (auto simp add: emptyset_regular epsilon_regular)
-  moreover have "eval ?f' s = eval (Var y) s" for s :: "'a state" using False by simp
+  moreover have "eval ?f' v = eval (Var y) v" for v :: "'a valuation" using False by simp
   moreover have "vars ?f' = vars (Var y) \<union> {x}" by simp
   ultimately show ?thesis by metis
 qed
@@ -50,28 +50,28 @@ qed
 lemma regular_fun_regular_fun'_Const:
   assumes "\<exists>r. Regular_Exp.lang r = l"
     shows "\<exists>f'. regular_fun' x f' \<and> vars f' = vars (Const l) \<union> {x}
-                \<and> (\<forall>s. parikh_img (eval (Const l) s) = parikh_img (eval f' s))"
+                \<and> (\<forall>v. parikh_img (eval (Const l) v) = parikh_img (eval f' v))"
 proof -
   let ?f' = "Union2 (Const l) (Concat (Const {}) (Var x))"
   have "regular_fun' x ?f'"
     unfolding regular_fun'_def using assms by (auto simp add: emptyset_regular)
-  moreover have "eval ?f' s = eval (Const l) s" for s :: "'a state" by simp
+  moreover have "eval ?f' v = eval (Const l) v" for v :: "'a valuation" by simp
   moreover have "vars ?f' = vars (Const l) \<union> {x}" by simp 
   ultimately show ?thesis by metis
 qed
 
 lemma regular_fun_regular_fun'_Union2:
   assumes "\<exists>f'. regular_fun' x f' \<and> vars f' = vars f1 \<union> {x} \<and>
-                (\<forall>s. parikh_img (eval f1 s) = parikh_img (eval f' s))"
+                (\<forall>v. parikh_img (eval f1 v) = parikh_img (eval f' v))"
           "\<exists>f'. regular_fun' x f' \<and> vars f' = vars f2 \<union> {x} \<and>
-                (\<forall>s. parikh_img (eval f2 s) = parikh_img (eval f' s))"
+                (\<forall>v. parikh_img (eval f2 v) = parikh_img (eval f' v))"
     shows "\<exists>f'. regular_fun' x f' \<and> vars f' = vars (Union2 f1 f2) \<union> {x} \<and>
-                (\<forall>s. parikh_img (eval (Union2 f1 f2) s) = parikh_img (eval f' s))"
+                (\<forall>v. parikh_img (eval (Union2 f1 f2) v) = parikh_img (eval f' v))"
 proof -
   from assms obtain f1' f2' where f1'_intro: "regular_fun' x f1' \<and> vars f1' = vars f1 \<union> {x} \<and>
-      (\<forall>s. parikh_img (eval f1 s) = parikh_img (eval f1' s))"
+      (\<forall>v. parikh_img (eval f1 v) = parikh_img (eval f1' v))"
     and f2'_intro: "regular_fun' x f2' \<and> vars f2' = vars f2 \<union> {x} \<and>
-      (\<forall>s. parikh_img (eval f2 s) = parikh_img (eval f2' s))"
+      (\<forall>v. parikh_img (eval f2 v) = parikh_img (eval f2' v))"
     by auto
   then obtain p1 q1 p2 q2 where p1_q1_intro: "regular_fun p1 \<and> regular_fun q1 \<and>
     f1' = Union2 p1 (Concat q1 (Var x)) \<and> (\<forall>y \<in> vars p1. y \<noteq> x)"
@@ -80,7 +80,7 @@ proof -
 
   let ?f' = "Union2 (Union2 p1 p2) (Concat (Union2 q1 q2) (Var x))"
   have "regular_fun' x ?f'" unfolding regular_fun'_def using p1_q1_intro p2_q2_intro by auto
-  moreover have "parikh_img (eval ?f' s) = parikh_img (eval (Union2 f1 f2) s)" for s
+  moreover have "parikh_img (eval ?f' v) = parikh_img (eval (Union2 f1 f2) v)" for v
     using p1_q1_intro p2_q2_intro f1'_intro f2'_intro
     by (simp add: conc_Un_distrib(2) sup_assoc sup_left_commute)
   moreover from f1'_intro f2'_intro p1_q1_intro p2_q2_intro
@@ -90,16 +90,16 @@ qed
 
 lemma regular_fun_regular_fun'_Concat:
   assumes "\<exists>f'. regular_fun' x f' \<and> vars f' = vars f1 \<union> {x} \<and>
-                (\<forall>s. parikh_img (eval f1 s) = parikh_img (eval f' s))"
+                (\<forall>v. parikh_img (eval f1 v) = parikh_img (eval f' v))"
           "\<exists>f'. regular_fun' x f' \<and> vars f' = vars f2 \<union> {x} \<and>
-                (\<forall>s. parikh_img (eval f2 s) = parikh_img (eval f' s))"
+                (\<forall>v. parikh_img (eval f2 v) = parikh_img (eval f' v))"
     shows "\<exists>f'. regular_fun' x f' \<and> vars f' = vars (Concat f1 f2) \<union> {x} \<and>
-                (\<forall>s. parikh_img (eval (Concat f1 f2) s) = parikh_img (eval f' s))"
+                (\<forall>v. parikh_img (eval (Concat f1 f2) v) = parikh_img (eval f' v))"
 proof -
   from assms obtain f1' f2' where f1'_intro: "regular_fun' x f1' \<and> vars f1' = vars f1 \<union> {x} \<and>
-      (\<forall>s. parikh_img (eval f1 s) = parikh_img (eval f1' s))"
+      (\<forall>v. parikh_img (eval f1 v) = parikh_img (eval f1' v))"
     and f2'_intro: "regular_fun' x f2' \<and> vars f2' = vars f2 \<union> {x} \<and>
-      (\<forall>s. parikh_img (eval f2 s) = parikh_img (eval f2' s))"
+      (\<forall>v. parikh_img (eval f2 v) = parikh_img (eval f2' v))"
     by auto
   then obtain p1 q1 p2 q2 where p1_q1_intro: "regular_fun p1 \<and> regular_fun q1 \<and>
     f1' = Union2 p1 (Concat q1 (Var x)) \<and> (\<forall>y \<in> vars p1. y \<noteq> x)"
@@ -109,29 +109,29 @@ proof -
   let ?q' = "Union2 (Concat q1 (Concat (Var x) q2)) (Union2 (Concat p1 q2) (Concat q1 p2))"
   let ?f' = "Union2 (Concat p1 p2) (Concat ?q' (Var x))"
 
-  have "\<forall>s. (parikh_img (eval (Concat f1 f2) s) = parikh_img (eval ?f' s))"
+  have "\<forall>v. (parikh_img (eval (Concat f1 f2) v) = parikh_img (eval ?f' v))"
   proof (rule allI)
-    fix s
-    have f2_subst: "parikh_img (eval f2 s) = parikh_img (eval p2 s \<union> eval q2 s @@ s x)"
+    fix v
+    have f2_subst: "parikh_img (eval f2 v) = parikh_img (eval p2 v \<union> eval q2 v @@ v x)"
       using p2_q2_intro f2'_intro by auto
 
-    have "parikh_img (eval (Concat f1 f2) s) = parikh_img ((eval p1 s \<union> eval q1 s @@ s x) @@ eval f2 s)"
+    have "parikh_img (eval (Concat f1 f2) v) = parikh_img ((eval p1 v \<union> eval q1 v @@ v x) @@ eval f2 v)"
       using p1_q1_intro f1'_intro
       by (metis eval.simps(1) eval.simps(3) eval.simps(5) parikh_conc_right)
-    also have "\<dots> = parikh_img (eval p1 s @@ eval f2 s \<union> eval q1 s @@ s x @@ eval f2 s)"
+    also have "\<dots> = parikh_img (eval p1 v @@ eval f2 v \<union> eval q1 v @@ v x @@ eval f2 v)"
       by (simp add: conc_Un_distrib(2) conc_assoc)
-    also have "\<dots> = parikh_img (eval p1 s @@ (eval p2 s \<union> eval q2 s @@ s x)
-        \<union> eval q1 s @@ s x @@ (eval p2 s \<union> eval q2 s @@ s x))"
+    also have "\<dots> = parikh_img (eval p1 v @@ (eval p2 v \<union> eval q2 v @@ v x)
+        \<union> eval q1 v @@ v x @@ (eval p2 v \<union> eval q2 v @@ v x))"
       using f2_subst by (smt (verit, ccfv_threshold) parikh_conc_right parikh_img_Un parikh_img_commut)
-    also have "\<dots> = parikh_img (eval p1 s @@ eval p2 s \<union> (eval p1 s @@ eval q2 s @@ s x \<union>
-        eval q1 s @@ eval p2 s @@ s x \<union> eval q1 s @@ s x @@ eval q2 s @@ s x))"
+    also have "\<dots> = parikh_img (eval p1 v @@ eval p2 v \<union> (eval p1 v @@ eval q2 v @@ v x \<union>
+        eval q1 v @@ eval p2 v @@ v x \<union> eval q1 v @@ v x @@ eval q2 v @@ v x))"
       using parikh_img_commut by (smt (z3) conc_Un_distrib(1) parikh_conc_right parikh_img_Un sup_assoc)
-    also have "\<dots> = parikh_img (eval p1 s @@ eval p2 s \<union> (eval p1 s @@ eval q2 s \<union>
-        eval q1 s @@ eval p2 s \<union> eval q1 s @@ s x @@ eval q2 s) @@ s x)"
+    also have "\<dots> = parikh_img (eval p1 v @@ eval p2 v \<union> (eval p1 v @@ eval q2 v \<union>
+        eval q1 v @@ eval p2 v \<union> eval q1 v @@ v x @@ eval q2 v) @@ v x)"
       by (simp add: conc_Un_distrib(2) conc_assoc)
-    also have "\<dots> = parikh_img (eval ?f' s)"
+    also have "\<dots> = parikh_img (eval ?f' v)"
       by (simp add: Un_commute)
-    finally show "parikh_img (eval (Concat f1 f2) s) = parikh_img (eval ?f' s)" .
+    finally show "parikh_img (eval (Concat f1 f2) v) = parikh_img (eval ?f' v)" .
   qed
   moreover have "regular_fun' x ?f'" unfolding regular_fun'_def using p1_q1_intro p2_q2_intro by auto
   moreover from f1'_intro f2'_intro p1_q1_intro p2_q2_intro
@@ -141,38 +141,38 @@ qed
 
 lemma regular_fun_regular_fun'_Star:
   assumes "\<exists>f'. regular_fun' x f' \<and> vars f' = vars f \<union> {x}
-                \<and> (\<forall>s. parikh_img (eval f s) = parikh_img (eval f' s))"
+                \<and> (\<forall>v. parikh_img (eval f v) = parikh_img (eval f' v))"
   shows "\<exists>f'. regular_fun' x f' \<and> vars f' = vars (Star f) \<union> {x}
-                \<and> (\<forall>s. parikh_img (eval (Star f) s) = parikh_img (eval f' s))"
+                \<and> (\<forall>v. parikh_img (eval (Star f) v) = parikh_img (eval f' v))"
 proof -
   from assms obtain f' where f'_intro: "regular_fun' x f' \<and> vars f' = vars f \<union> {x} \<and>
-      (\<forall>s. parikh_img (eval f s) = parikh_img (eval f' s))" by auto
+      (\<forall>v. parikh_img (eval f v) = parikh_img (eval f' v))" by auto
   then obtain p q where p_q_intro: "regular_fun p \<and> regular_fun q \<and>
     f' = Union2 p (Concat q (Var x)) \<and> (\<forall>y \<in> vars p. y \<noteq> x)" unfolding regular_fun'_def by auto
 
   let ?q_new = "Concat (Star p) (Concat (Star (Concat q (Var x))) (Concat (Star (Concat q (Var x))) q))"
   let ?f_new = "Union2 (Star p) (Concat ?q_new (Var x))"
 
-  have "\<forall>s. (parikh_img (eval (Star f) s) = parikh_img (eval ?f_new s))"
+  have "\<forall>v. (parikh_img (eval (Star f) v) = parikh_img (eval ?f_new v))"
   proof (rule allI)
-    fix s
-    have "parikh_img (eval (Star f) s) = parikh_img (star (eval p s \<union> eval q s @@ s x))"
+    fix v
+    have "parikh_img (eval (Star f) v) = parikh_img (star (eval p v \<union> eval q v @@ v x))"
       using f'_intro parikh_star_mono_eq p_q_intro
       by (metis eval.simps(1) eval.simps(3) eval.simps(5) eval.simps(6))
-    also have "\<dots> = parikh_img (star (eval p s) @@ star (eval q s @@ s x))"
+    also have "\<dots> = parikh_img (star (eval p v) @@ star (eval q v @@ v x))"
       using parikh_img_star by blast
-    also have "\<dots> = parikh_img (star (eval p s) @@
-        star ({[]} \<union> star (eval q s @@ s x) @@ eval q s @@ s x))"
+    also have "\<dots> = parikh_img (star (eval p v) @@
+        star ({[]} \<union> star (eval q v @@ v x) @@ eval q v @@ v x))"
       by (metis Un_commute conc_star_comm star_idemp star_unfold_left)
-    also have "\<dots> = parikh_img (star (eval p s) @@ star (star (eval q s @@ s x) @@ eval q s @@ s x))"
+    also have "\<dots> = parikh_img (star (eval p v) @@ star (star (eval q v @@ v x) @@ eval q v @@ v x))"
       by auto
-    also have "\<dots> = parikh_img (star (eval p s) @@ ({[]} \<union> star (eval q s @@ s x)
-        @@ star (eval q s @@ s x) @@ eval q s @@ s x))"
+    also have "\<dots> = parikh_img (star (eval p v) @@ ({[]} \<union> star (eval q v @@ v x)
+        @@ star (eval q v @@ v x) @@ eval q v @@ v x))"
       using parikh_img_star2 parikh_conc_left by blast
-    also have "\<dots> = parikh_img (star (eval p s) @@ {[]} \<union> star (eval p s) @@ star (eval q s @@ s x)
-        @@ star (eval q s @@ s x) @@ eval q s @@ s x)" by (metis conc_Un_distrib(1))
-    also have "\<dots> = parikh_img (eval ?f_new s)" by (simp add: conc_assoc)
-    finally show "parikh_img (eval (Star f) s) = parikh_img (eval ?f_new s)" .
+    also have "\<dots> = parikh_img (star (eval p v) @@ {[]} \<union> star (eval p v) @@ star (eval q v @@ v x)
+        @@ star (eval q v @@ v x) @@ eval q v @@ v x)" by (metis conc_Un_distrib(1))
+    also have "\<dots> = parikh_img (eval ?f_new v)" by (simp add: conc_assoc)
+    finally show "parikh_img (eval (Star f) v) = parikh_img (eval ?f_new v)" .
   qed
   moreover have "regular_fun' x ?f_new" unfolding regular_fun'_def using p_q_intro by fastforce
   moreover from f'_intro p_q_intro have "vars ?f_new = vars (Star f) \<union> {x}" by auto
@@ -219,13 +219,13 @@ locale of_form_regular_fun' =
 begin
 
 abbreviation "eq \<equiv> Union2 p (Concat q (Var x))"
-abbreviation "sol \<equiv> Concat (Star (subst q (Var(x := p)))) p"
+abbreviation "sol \<equiv> Concat (Star (subst (Var(x := p)) q)) p"
 
 
 (* F(E)*E is a regular function *)
 lemma sol_is_reg: "regular_fun sol"
 proof -
-  from p_reg q_reg have r_reg: "regular_fun (subst q (Var(x := p)))"
+  from p_reg q_reg have r_reg: "regular_fun (subst (Var(x := p)) q)"
     using subst_reg_fun_update by auto
   with p_reg show "regular_fun sol" by fast
 qed
@@ -235,7 +235,7 @@ qed
 lemma sol_vars: "vars sol \<subseteq> vars eq - {x}"
 proof -
   let ?upd = "Var(x := p)"
-  let ?subst_q = "subst q ?upd"
+  let ?subst_q = "subst ?upd q"
   from x_not_in_p have vars_p: "vars p \<subseteq> vars eq - {x}" by fastforce
 
   have "vars ?subst_q \<subseteq> vars eq - {x}"
@@ -260,57 +260,57 @@ qed
 (* F(E)*E is a solution of equation (3) from the paper (with \<supseteq> instead of =) *)
 lemma sol_is_sol_ineq: "partial_sol_ineq x eq sol"
 unfolding partial_sol_ineq_def proof (rule allI, rule impI)
-  fix s
-  assume x_is_sol: "s x = eval sol s"
+  fix v
+  assume x_is_sol: "v x = eval sol v"
 
-  let ?r = "subst q (Var (x := p))"
+  let ?r = "subst (Var (x := p)) q"
   let ?upd = "Var(x := sol)"
-  let ?q_subst = "subst q ?upd"
-  let ?eq_subst = "subst eq ?upd"
+  let ?q_subst = "subst ?upd q"
+  let ?eq_subst = "subst ?upd eq"
 
   from sol_is_reg have r_reg: "regular_fun ?r" unfolding fun_upd_def by blast
-  have homogeneous_app: "parikh_img (eval ?q_subst s) \<subseteq> parikh_img (eval (Concat (Star ?r) ?r) s)"
+  have homogeneous_app: "parikh_img (eval ?q_subst v) \<subseteq> parikh_img (eval (Concat (Star ?r) ?r) v)"
     using reg_fun_homogeneous[OF q_reg r_reg p_reg] by blast
 
-  from x_not_in_p have "eval (subst p ?upd) s = eval p s" using eval_vars_subst[of p] by simp
-  then have "parikh_img (eval ?eq_subst s) = parikh_img (eval p s \<union> eval ?q_subst s @@ eval sol s)"
+  from x_not_in_p have "eval (subst ?upd p) v = eval p v" using eval_vars_subst[of p] by simp
+  then have "parikh_img (eval ?eq_subst v) = parikh_img (eval p v \<union> eval ?q_subst v @@ eval sol v)"
     by simp
-  also have "\<dots> \<subseteq> parikh_img (eval p s \<union> eval (Concat (Star ?r) ?r) s @@ eval sol s)"
+  also have "\<dots> \<subseteq> parikh_img (eval p v \<union> eval (Concat (Star ?r) ?r) v @@ eval sol v)"
     using homogeneous_app by (metis dual_order.refl parikh_conc_right_subset parikh_img_Un sup.mono)
-  also have "\<dots> = parikh_img (eval p s) \<union>
-      parikh_img (star (eval ?r s) @@ eval ?r s @@ star (eval ?r s) @@ eval p s)"
+  also have "\<dots> = parikh_img (eval p v) \<union>
+      parikh_img (star (eval ?r v) @@ eval ?r v @@ star (eval ?r v) @@ eval p v)"
     by (simp add: conc_assoc)
-  also have "\<dots> = parikh_img (eval p s) \<union>
-      parikh_img (eval ?r s @@ star (eval ?r s) @@ eval p s)"
+  also have "\<dots> = parikh_img (eval p v) \<union>
+      parikh_img (eval ?r v @@ star (eval ?r v) @@ eval p v)"
     using parikh_img_commut conc_star_star by (smt (verit, best) conc_assoc conc_star_comm)
-  also have "\<dots> = parikh_img (star (eval ?r s) @@ eval p s)"
+  also have "\<dots> = parikh_img (star (eval ?r v) @@ eval p v)"
     using star_unfold_left
     by (smt (verit) conc_Un_distrib(2) conc_assoc conc_epsilon(1) parikh_img_Un sup_commute)
-  finally have *: "parikh_img (eval ?eq_subst s) \<subseteq> parikh_img (s x)" using x_is_sol by simp
+  finally have *: "parikh_img (eval ?eq_subst v) \<subseteq> parikh_img (v x)" using x_is_sol by simp
 
-  from x_is_sol have "s = s(x := eval sol s)" using fun_upd_triv by metis
-  then have "eval eq s = eval (subst eq (Var(x := sol))) s"
-    using substitution_lemma_update[of eq] by presburger
-  with * show "solves_ineq_comm x eq s" unfolding solves_ineq_comm_def by argo
+  from x_is_sol have "v = v(x := eval sol v)" using fun_upd_triv by metis
+  then have "eval eq v = eval (subst (Var(x := sol)) eq) v"
+    using substitution_lemma_update[where f=eq] by presburger
+  with * show "solves_ineq_comm x eq v" unfolding solves_ineq_comm_def by argo
 qed
 
 
 lemma sol_is_minimal:
-  assumes is_sol:    "solves_ineq_comm x eq s"
-      and sol'_s:    "s x = eval sol' s"
-    shows            "parikh_img (eval sol s) \<subseteq> parikh_img (s x)"
+  assumes is_sol:    "solves_ineq_comm x eq v"
+      and sol'_s:    "v x = eval sol' v"
+    shows            "parikh_img (eval sol v) \<subseteq> parikh_img (v x)"
 proof -
-  from is_sol sol'_s have is_sol': "parikh_img (eval q s @@ s x \<union> eval p s) \<subseteq> parikh_img (s x)"
+  from is_sol sol'_s have is_sol': "parikh_img (eval q v @@ v x \<union> eval p v) \<subseteq> parikh_img (v x)"
     unfolding solves_ineq_comm_def by simp
-  then have 1: "parikh_img (eval (Concat (Star q) p) s) \<subseteq> parikh_img (s x)"
+  then have 1: "parikh_img (eval (Concat (Star q) p) v) \<subseteq> parikh_img (v x)"
     using parikh_img_arden by auto
 
-  from is_sol' have "parikh_img (eval p s) \<subseteq> parikh_img (eval (Var x) s)" by auto
-  then have "parikh_img (eval (subst q (Var(x := p))) s) \<subseteq> parikh_img (eval q s)"
+  from is_sol' have "parikh_img (eval p v) \<subseteq> parikh_img (eval (Var x) v)" by auto
+  then have "parikh_img (eval (subst (Var(x := p)) q) v) \<subseteq> parikh_img (eval q v)"
     using parikh_img_subst_mono_upd by (metis fun_upd_triv subst_id)
-  then have "parikh_img (eval (Star (subst q (Var(x := p)))) s) \<subseteq> parikh_img (eval (Star q) s)"
+  then have "parikh_img (eval (Star (subst (Var(x := p)) q)) v) \<subseteq> parikh_img (eval (Star q) v)"
     using parikh_star_mono by auto
-  then have "parikh_img (eval sol s) \<subseteq> parikh_img (eval (Concat (Star q) p) s)"
+  then have "parikh_img (eval sol v) \<subseteq> parikh_img (eval (Concat (Star q) p) v)"
     using parikh_conc_right_subset by (metis eval.simps(5))
 
   with 1 show ?thesis by fast
@@ -359,12 +359,12 @@ lemma exists_minimal_reg_sol:
 proof -
   from regular_fun_regular_fun'[OF eq_reg] obtain eq'
     where eq'_intro: "regular_fun' x eq' \<and> vars eq' = vars eq \<union> {x} \<and>
-                    (\<forall>s. parikh_img (eval eq s) = parikh_img (eval eq' s))" by blast
+                    (\<forall>v. parikh_img (eval eq v) = parikh_img (eval eq' v))" by blast
   then obtain p q
     where p_q_intro: "regular_fun p \<and> regular_fun q \<and> eq' = Union2 p (Concat q (Var x)) \<and> x \<notin> vars p"
     unfolding regular_fun'_def by blast
 
-  let ?sol = "Concat (Star (subst q (Var(x := p)))) p"
+  let ?sol = "Concat (Star (subst (Var(x := p)) q)) p"
   from p_q_intro have sol_prop: "regular_fun ?sol \<and> partial_min_sol_one_ineq x eq' ?sol"
     using of_form_regular_fun'.sol_is_minimal_reg_sol unfolding of_form_regular_fun'_def by blast
   with eq'_intro have "partial_min_sol_one_ineq x eq ?sol"
@@ -385,13 +385,13 @@ locale minimal_sol_one_eq =
       and r_valid:      "r < length sys"
       and sols_is_sol:  "partial_min_sol_ineq_sys r sys sols"
       and sols_reg:     "\<forall>i. regular_fun (sols i)"
-      and sol_r_is_sol: "partial_min_sol_one_ineq r (sys_subst sys sols ! r) sol_r"
+      and sol_r_is_sol: "partial_min_sol_one_ineq r (subst_sys sols sys ! r) sol_r"
       and sol_r_reg:    "regular_fun sol_r"
 begin
 
 
-abbreviation "sys' \<equiv> sys_subst sys sols"
-abbreviation "sols' \<equiv> \<lambda>i. subst (sols i) (Var(r := sol_r))"
+abbreviation "sys' \<equiv> subst_sys sols sys"
+abbreviation "sols' \<equiv> \<lambda>i. subst (Var(r := sol_r)) (sols i)"
 
 
 lemma sols'_r: "sols' r = sol_r"
@@ -404,52 +404,52 @@ lemma sols'_reg: "\<forall>i. regular_fun (sols' i)"
 
 lemma sols'_is_sol: "solution_ineq_sys (take (Suc r) sys) sols'"
 unfolding solution_ineq_sys_def proof (rule allI, rule impI)
-  fix s
-  assume s_sols': "\<forall>x. s x = eval (sols' x) s"
+  fix v
+  assume s_sols': "\<forall>x. v x = eval (sols' x) v"
 
-  from sols'_r s_sols' have s_r_sol_r: "s r = eval sol_r s" by simp
-  with s_sols' have s_sols: "s x = eval (sols x) s" for x
-    using substitution_lemma_update[of "sols x"] by (auto simp add: fun_upd_idem)
-  with sols_is_sol have solves_r_sys: "solves_ineq_sys_comm (take r sys) s"
+  from sols'_r s_sols' have s_r_sol_r: "v r = eval sol_r v" by simp
+  with s_sols' have s_sols: "v x = eval (sols x) v" for x
+    using substitution_lemma_update[where f="sols x"] by (auto simp add: fun_upd_idem)
+  with sols_is_sol have solves_r_sys: "solves_ineq_sys_comm (take r sys) v"
     unfolding partial_min_sol_ineq_sys_def solution_ineq_sys_def by meson
 
-  have "eval (sys ! r) (\<lambda>y. eval (sols y) s) = eval (sys' ! r) s"
-    using substitution_lemma[of "\<lambda>y. eval (sols y) s"]
-    by (simp add: r_valid Suc_le_lessD sys_subst_subst)
-  with s_sols have "eval (sys ! r) s = eval (sys' ! r) s"
+  have "eval (sys ! r) (\<lambda>y. eval (sols y) v) = eval (sys' ! r) v"
+    using substitution_lemma[of "\<lambda>y. eval (sols y) v"]
+    by (simp add: r_valid Suc_le_lessD subst_sys_subst)
+  with s_sols have "eval (sys ! r) v = eval (sys' ! r) v"
     by (metis (mono_tags, lifting) eval_vars)
-  with sol_r_is_sol s_r_sol_r have "parikh_img (eval (sys ! r) s) \<subseteq> parikh_img (s r)"
+  with sol_r_is_sol s_r_sol_r have "parikh_img (eval (sys ! r) v) \<subseteq> parikh_img (v r)"
     unfolding partial_min_sol_one_ineq_def partial_sol_ineq_def solves_ineq_comm_def by simp
-  with solves_r_sys show "solves_ineq_sys_comm (take (Suc r) sys) s"
+  with solves_r_sys show "solves_ineq_sys_comm (take (Suc r) sys) v"
     unfolding solves_ineq_sys_comm_def solves_ineq_comm_def by (auto simp add: less_Suc_eq)
 qed
 
 
-lemma sols'_min: "\<forall>sols2 s2. (\<forall>x. s2 x = eval (sols2 x) s2)
-                   \<and> solves_ineq_sys_comm (take (Suc r) sys) s2
-                   \<longrightarrow> (\<forall>i. parikh_img (eval (sols' i) s2) \<subseteq> parikh_img (s2 i))"
+lemma sols'_min: "\<forall>sols2 v2. (\<forall>x. v2 x = eval (sols2 x) v2)
+                   \<and> solves_ineq_sys_comm (take (Suc r) sys) v2
+                   \<longrightarrow> (\<forall>i. parikh_img (eval (sols' i) v2) \<subseteq> parikh_img (v2 i))"
 proof (rule allI | rule impI)+
-  fix sols2 s2 i
-  assume as: "(\<forall>x. s2 x = eval (sols2 x) s2) \<and> solves_ineq_sys_comm (take (Suc r) sys) s2"
+  fix sols2 v2 i
+  assume as: "(\<forall>x. v2 x = eval (sols2 x) v2) \<and> solves_ineq_sys_comm (take (Suc r) sys) v2"
 
-  then have "solves_ineq_sys_comm (take r sys) s2" unfolding solves_ineq_sys_comm_def by fastforce
-  with as sols_is_sol have sols_s2: "parikh_img (eval (sols i) s2) \<subseteq> parikh_img (s2 i)" for i
+  then have "solves_ineq_sys_comm (take r sys) v2" unfolding solves_ineq_sys_comm_def by fastforce
+  with as sols_is_sol have sols_s2: "parikh_img (eval (sols i) v2) \<subseteq> parikh_img (v2 i)" for i
     unfolding partial_min_sol_ineq_sys_def by auto
 
-  have "eval (sys' ! r) s2 = eval (sys ! r) (\<lambda>i. eval (sols i) s2)"
-    unfolding sys_subst_def using substitution_lemma[where f="sys ! r"]
+  have "eval (sys' ! r) v2 = eval (sys ! r) (\<lambda>i. eval (sols i) v2)"
+    unfolding subst_sys_def using substitution_lemma[where f="sys ! r"]
     by (simp add: r_valid Suc_le_lessD)
-  with sols_s2 have "parikh_img (eval (sys' ! r) s2) \<subseteq> parikh_img (eval (sys ! r) s2)"
+  with sols_s2 have "parikh_img (eval (sys' ! r) v2) \<subseteq> parikh_img (eval (sys ! r) v2)"
     using lfun_mono_parikh[of "sys ! r"] by auto
-  with as have "solves_ineq_comm r (sys' ! r) s2"
+  with as have "solves_ineq_comm r (sys' ! r) v2"
     unfolding solves_ineq_sys_comm_def solves_ineq_comm_def using r_valid by force
-  with as sol_r_is_sol have sol_r_min: "parikh_img (eval sol_r s2) \<subseteq> parikh_img (s2 r)"
+  with as sol_r_is_sol have sol_r_min: "parikh_img (eval sol_r v2) \<subseteq> parikh_img (v2 r)"
     unfolding partial_min_sol_one_ineq_def by blast
 
-  let ?s' = "s2(r := eval sol_r s2)"
-  from sol_r_min have "parikh_img (?s' i) \<subseteq> parikh_img (s2 i)" for i by simp
-  with sols_s2 show "parikh_img (eval (sols' i) s2) \<subseteq> parikh_img (s2 i)"
-    using substitution_lemma_update[of "sols i"] lfun_mono_parikh[of "sols i" ?s' s2] by force
+  let ?v' = "v2(r := eval sol_r v2)"
+  from sol_r_min have "parikh_img (?v' i) \<subseteq> parikh_img (v2 i)" for i by simp
+  with sols_s2 show "parikh_img (eval (sols' i) v2) \<subseteq> parikh_img (v2 i)"
+    using substitution_lemma_update[where f="sols i"] lfun_mono_parikh[of "sols i" ?v' v2] by force
 qed
 
 
@@ -463,10 +463,10 @@ proof -
     unfolding partial_min_sol_ineq_sys_def by simp
   with sols_is_sol have vars_sols: "\<forall>i < length sys. \<forall>x \<in> vars (sols i). x \<ge> r \<and> x < length sys"
     unfolding partial_min_sol_ineq_sys_def by (metis empty_iff insert_iff leI vars.simps(1))
-  with sys_valid have "\<forall>x \<in> vars (subst (sys ! i) sols). x \<ge> r \<and> x < length sys" if "i < length sys" for i
-    using vars_subst[of "sys ! i" sols] that by (metis UN_E nth_mem)
+  with sys_valid have "\<forall>x \<in> vars (subst sols (sys ! i)). x \<ge> r \<and> x < length sys" if "i < length sys" for i
+    using vars_subst[of sols "sys ! i"] that by (metis UN_E nth_mem)
   then have "\<forall>x \<in> vars (sys' ! i). x \<ge> r \<and> x < length sys" if "i < length sys" for i
-    unfolding sys_subst_def using r_valid that by auto
+    unfolding subst_sys_def using r_valid that by auto
   moreover from sol_r_is_sol have "vars (sol_r) \<subseteq> vars (sys' ! r) - {r}"
     unfolding partial_min_sol_one_ineq_def by simp
   ultimately have vars_sol_r: "\<forall>x \<in> vars sol_r. x > r \<and> x < length sys"
@@ -508,10 +508,10 @@ next
   then obtain sols where sols_intro: "partial_min_sol_ineq_sys r sys sols \<and> (\<forall>i. regular_fun (sols i))"
     by auto
 
-  let ?sys' = "sys_subst sys sols"
+  let ?sys' = "subst_sys sols sys"
   from eqs_reg Suc.prems have "regular_fun (sys ! r)" by simp
   with sols_intro Suc.prems have sys_r_reg: "regular_fun (?sys' ! r)"
-    using subst_reg_fun[of "sys ! r"] sys_subst_subst[of r sys] by simp
+    using subst_reg_fun[of "sys ! r"] subst_sys_subst[of r sys] by simp
   then obtain sol_r where sol_r_intro:
     "regular_fun sol_r \<and> partial_min_sol_one_ineq r (?sys' ! r) sol_r"
     using exists_minimal_reg_sol by blast
@@ -535,14 +535,14 @@ proof -
     by blast
   then have "const_fun (sols i)" if "i < length sys" for i
     using that unfolding partial_min_sol_ineq_sys_def by (meson equals0I leD)
-  with sols_intro have "\<exists>l. regular_lang l \<and> (\<forall>s. eval (sols i) s = l)" if "i < length sys" for i
+  with sols_intro have "\<exists>l. regular_lang l \<and> (\<forall>v. eval (sols i) v = l)" if "i < length sys" for i
     using that const_fun_regular_lang by metis
-  then obtain ls where ls_intro: "\<forall>i < length sys. regular_lang (ls i) \<and> (\<forall>s. eval (sols i) s = ls i)"
+  then obtain ls where ls_intro: "\<forall>i < length sys. regular_lang (ls i) \<and> (\<forall>v. eval (sols i) v = ls i)"
     by metis
 
   let ?ls' = "\<lambda>i. if i < length sys then ls i else {}"
   from ls_intro have ls'_intro:
-    "(\<forall>i < length sys. regular_lang (?ls' i) \<and> (\<forall>s. eval (sols i) s = ?ls' i))
+    "(\<forall>i < length sys. regular_lang (?ls' i) \<and> (\<forall>v. eval (sols i) v = ?ls' i))
      \<and> (\<forall>i \<ge> length sys. ?ls' i = {})" by force
   then have ls'_regular: "regular_lang (?ls' i)" for i by (meson lang.simps(1))
 
