Parikh/Pilling_Lemma.thy
@@ -15,57 +15,57 @@ subsection \<open>g_pre (in the paper g_{iN} resp. X_{iN}\<close>
 
 fun g_pre :: "'a eq_sys \<Rightarrow> nat \<Rightarrow> nat \<Rightarrow> 'a lfun" where
   "g_pre _ _ 0 = Const {}" |
-  "g_pre f_sys i (Suc n) = subst (f_sys ! i) (\<lambda>j. if j < length f_sys then g_pre f_sys j n else Var j)"
+  "g_pre f_sys i (Suc n) = subst (\<lambda>j. if j < length f_sys then g_pre f_sys j n else Var j) (f_sys ! i)"
 
 
 lemma g_pre_eval:
-  assumes "\<forall>j < length f_sys. s' j = eval (g_pre f_sys j n) s"
-      and "\<forall>j \<ge> length f_sys. s' j = s j"
-    shows "eval (g_pre f_sys i (Suc n)) s = eval (f_sys ! i) s'"
+  assumes "\<forall>j < length f_sys. v' j = eval (g_pre f_sys j n) v"
+      and "\<forall>j \<ge> length f_sys. v' j = v j"
+    shows "eval (g_pre f_sys i (Suc n)) v = eval (f_sys ! i) v'"
 using assms by (simp add: substitution_lemma)
 
 
 lemma g_pre_monotonically_increasing:
-  "eval (g_pre f_sys i n) s \<subseteq> eval (g_pre f_sys i (Suc n)) s"
+  "eval (g_pre f_sys i n) v \<subseteq> eval (g_pre f_sys i (Suc n)) v"
 proof (induction n arbitrary: i)
   case 0
   then show ?case by auto
 next
   case (Suc n)
-  let ?s = "\<lambda>j. if j < length f_sys then eval (g_pre f_sys j n) s else s j"
-  let ?s_Suc = "\<lambda>j. if j < length f_sys then eval (g_pre f_sys j (Suc n)) s else s j"
-  from Suc.IH have s_subseteq_s_Suc: "?s j \<subseteq> ?s_Suc j" for j by auto
+  let ?v = "\<lambda>j. if j < length f_sys then eval (g_pre f_sys j n) v else v j"
+  let ?v_Suc = "\<lambda>j. if j < length f_sys then eval (g_pre f_sys j (Suc n)) v else v j"
+  from Suc.IH have v_subseteq_v_Suc: "?v j \<subseteq> ?v_Suc j" for j by auto
 
-  have "eval (g_pre f_sys i (Suc n)) s = eval (f_sys ! i) ?s" using g_pre_eval[of f_sys] by auto
-  also have "\<dots> \<subseteq> eval (f_sys ! i) ?s_Suc" using s_subseteq_s_Suc lfun_mono_aux[where s="?s"] by auto
-  also have "\<dots> = eval (g_pre f_sys i (Suc (Suc n))) s" using g_pre_eval[of f_sys ?s_Suc] by auto
+  have "eval (g_pre f_sys i (Suc n)) v = eval (f_sys ! i) ?v" using g_pre_eval[of f_sys] by auto
+  also have "\<dots> \<subseteq> eval (f_sys ! i) ?v_Suc" using v_subseteq_v_Suc lfun_mono_aux[where v="?v"] by auto
+  also have "\<dots> = eval (g_pre f_sys i (Suc (Suc n))) v" using g_pre_eval[of f_sys ?v_Suc] by auto
   finally show ?case .
 qed
 
 
 lemma g_pre_subseteq_sol:
   assumes "i < length f_sys"
-      and "solves_ineq_sys f_sys s"
-    shows "eval (g_pre f_sys i n) s \<subseteq> eval (f_sys ! i) s"
+      and "solves_ineq_sys f_sys v"
+    shows "eval (g_pre f_sys i n) v \<subseteq> eval (f_sys ! i) v"
 using assms proof (induction n arbitrary: i)
   case 0
   then show ?case by auto
 next
   case (Suc n)
-  let ?s' = "\<lambda>j. if j < length f_sys then eval (g_pre f_sys j n) s else s j"
+  let ?v' = "\<lambda>j. if j < length f_sys then eval (g_pre f_sys j n) v else v j"
 
-  have "?s' j \<subseteq> s j" for j
+  have "?v' j \<subseteq> v j" for j
   proof (cases "j < length f_sys")
     case True
-    with Suc have "?s' j \<subseteq> eval (f_sys ! j) s" by auto
-    also have "\<dots> \<subseteq> s j" using assms(2) True unfolding solves_ineq_sys_def by auto
+    with Suc have "?v' j \<subseteq> eval (f_sys ! j) v" by auto
+    also have "\<dots> \<subseteq> v j" using assms(2) True unfolding solves_ineq_sys_def by auto
     finally show ?thesis .
   next
     case False
     then show ?thesis by auto
   qed
-  then have "eval (f_sys ! i) ?s' \<subseteq> eval (f_sys ! i) s" using lfun_mono_aux by meson
-  then show ?case using g_pre_eval[of f_sys ?s'] by auto
+  then have "eval (f_sys ! i) ?v' \<subseteq> eval (f_sys ! i) v" using lfun_mono_aux by meson
+  then show ?case using g_pre_eval[of f_sys ?v'] by auto
 qed
 
 
@@ -100,12 +100,12 @@ unfolding g_def using assms g_pre_indep by auto
 
 lemma solves_g_if_solves_f_ineq:
   assumes "i < length f_sys"
-      and "solves_ineq_sys f_sys s"
-    shows "eval (g f_sys i) s \<subseteq> eval (f_sys ! i) s"
+      and "solves_ineq_sys f_sys v"
+    shows "eval (g f_sys i) v \<subseteq> eval (f_sys ! i) v"
 unfolding g_def proof
   fix x
-  assume "x \<in> eval (UnionC (g_pre f_sys i)) s"
-  then show "x \<in> eval (f_sys ! i) s" using g_pre_subseteq_sol[OF assms] by auto
+  assume "x \<in> eval (UnionC (g_pre f_sys i)) v"
+  then show "x \<in> eval (f_sys ! i) v" using g_pre_subseteq_sol[OF assms] by auto
 qed
 
 
@@ -131,27 +131,27 @@ proof
 qed
 
 
-lemma g_pre_g_Union: "(\<Union>n. eval (g_pre f_sys i (Suc n)) s) =
-  eval (subst (f_sys ! i) (\<lambda>i. if i < length f_sys then g f_sys i else Var i)) s"
+lemma g_pre_g_Union: "(\<Union>n. eval (g_pre f_sys i (Suc n)) v) =
+  eval (subst (\<lambda>i. if i < length f_sys then g f_sys i else Var i) (f_sys ! i)) v"
 proof -
-  let ?s = "(\<lambda>n j. if j < length f_sys then eval (g_pre f_sys j n) s else s j)"
-  have "?s n j \<subseteq> ?s (Suc n) j" for n j
+  let ?v = "(\<lambda>n j. if j < length f_sys then eval (g_pre f_sys j n) v else v j)"
+  have "?v n j \<subseteq> ?v (Suc n) j" for n j
     using g_pre_monotonically_increasing by fastforce
-  then have s_monotone: "\<forall>n. ?s n \<le> ?s (Suc n)" by (simp add: le_fun_def)
+  then have s_monotone: "\<forall>n. ?v n \<le> ?v (Suc n)" by (simp add: le_fun_def)
 
-  have s_Union: "(\<Union>i. if x < length f_sys then eval (g_pre f_sys x i) s else s x) =
-    (if x < length f_sys then eval (g f_sys x) s else s x)" for x
+  have s_Union: "(\<Union>i. if x < length f_sys then eval (g_pre f_sys x i) v else v x) =
+    (if x < length f_sys then eval (g f_sys x) v else v x)" for x
     unfolding g_def by simp
 
-  have "eval (g_pre f_sys i (Suc n)) s = eval (f_sys ! i) (?s n)" for n
+  have "eval (g_pre f_sys i (Suc n)) v = eval (f_sys ! i) (?v n)" for n
     using g_pre_eval[of f_sys] by auto
-  then have "(\<Union>n. eval (g_pre f_sys i (Suc n)) s) = (\<Union>n. eval (f_sys ! i) (?s n))" by auto
-  also have "\<dots> = eval (f_sys ! i) (\<lambda>x. \<Union>i. if x < length f_sys then eval (g_pre f_sys x i) s else s x)"
-    using s_monotone lfun_cont[of ?s "f_sys ! i"] by argo
-  also have "\<dots> = eval (f_sys ! i) (\<lambda>x. if x < length f_sys then eval (g f_sys x) s else s x)"
+  then have "(\<Union>n. eval (g_pre f_sys i (Suc n)) v) = (\<Union>n. eval (f_sys ! i) (?v n))" by auto
+  also have "\<dots> = eval (f_sys ! i) (\<lambda>x. \<Union>i. if x < length f_sys then eval (g_pre f_sys x i) v else v x)"
+    using s_monotone lfun_cont[of ?v "f_sys ! i"] by argo
+  also have "\<dots> = eval (f_sys ! i) (\<lambda>x. if x < length f_sys then eval (g f_sys x) v else v x)"
     using s_Union by simp
-  also have "\<dots> = eval (subst (f_sys ! i) (\<lambda>i. if i < length f_sys then g f_sys i else Var i)) s"
-    using substitution_lemma[of "\<lambda>x. if x < length f_sys then eval (g f_sys x) s else s x"
+  also have "\<dots> = eval (subst (\<lambda>i. if i < length f_sys then g f_sys i else Var i) (f_sys ! i)) v"
+    using substitution_lemma[of "\<lambda>x. if x < length f_sys then eval (g f_sys x) v else v x"
                                 "\<lambda>i. if i < length f_sys then g f_sys i else Var i"]
     by fastforce
   finally show ?thesis .
@@ -159,17 +159,17 @@ qed
 
 
 lemma solves_f_if_solves_g_eq:
-  assumes "\<forall>i < length f_sys. eval (g f_sys i) s = s i"
-  shows "solves_eq_sys f_sys s"
+  assumes "\<forall>i < length f_sys. eval (g f_sys i) v = v i"
+  shows "solves_eq_sys f_sys v"
 unfolding solves_eq_sys_def proof (standard, standard)
   fix i
   assume "i < length f_sys"
-  with assms(1) have "s i = (\<Union>n. eval (g_pre f_sys i n) s)" unfolding g_def by auto
-  also have "\<dots> = (\<Union>n. eval (g_pre f_sys i (Suc n)) s)"
-    using Union_index_shift[of "\<lambda>n. eval (g_pre f_sys i n) s"] by auto
-  also have "\<dots> = eval (f_sys ! i) s"
+  with assms(1) have "v i = (\<Union>n. eval (g_pre f_sys i n) v)" unfolding g_def by auto
+  also have "\<dots> = (\<Union>n. eval (g_pre f_sys i (Suc n)) v)"
+    using Union_index_shift[of "\<lambda>n. eval (g_pre f_sys i n) v"] by auto
+  also have "\<dots> = eval (f_sys ! i) v"
     using g_pre_g_Union[of f_sys] assms by (simp add: substitution_lemma)
-  finally show "eval (f_sys ! i) s = s i" by auto
+  finally show "eval (f_sys ! i) v = v i" by auto
 qed
 
 
@@ -177,20 +177,20 @@ qed
 lemma lemma_paper:
   assumes "\<forall>eq \<in> set f_sys. regular_fun eq"
     shows "\<exists>g_sys. length g_sys = length f_sys \<and> (\<forall>eq \<in> set g_sys. \<forall>x \<in> vars eq. x \<ge> length f_sys)
-                \<and> (\<forall>s. solves_ineq_sys f_sys s \<longrightarrow> solves_ineq_sys g_sys s)
-                \<and> (\<forall>s. solves_eq_sys g_sys s \<longrightarrow> solves_eq_sys f_sys s)"
+                \<and> (\<forall>v. solves_ineq_sys f_sys v \<longrightarrow> solves_ineq_sys g_sys v)
+                \<and> (\<forall>v. solves_eq_sys g_sys v \<longrightarrow> solves_eq_sys f_sys v)"
 proof -
   let ?g_sys = "map (\<lambda>i. g f_sys i) [0..<length f_sys]"
   have length_g_sys: "length ?g_sys = length f_sys" by auto
   have indep_g_sys: "\<forall>eq \<in> set ?g_sys. \<forall>x \<in> vars eq. x \<ge> length f_sys"
     using g_indep by fastforce
 
-  have "\<lbrakk> i < length f_sys; solves_ineq_sys f_sys s \<rbrakk> \<Longrightarrow> eval (?g_sys ! i) s \<subseteq> s i" for s i
+  have "\<lbrakk> i < length f_sys; solves_ineq_sys f_sys v \<rbrakk> \<Longrightarrow> eval (?g_sys ! i) v \<subseteq> v i" for v i
     using solves_g_if_solves_f_ineq solves_ineq_sys_def by fastforce
-  then have g_sol_of_f: "solves_ineq_sys f_sys s \<longrightarrow> solves_ineq_sys ?g_sys s" for s
+  then have g_sol_of_f: "solves_ineq_sys f_sys v \<longrightarrow> solves_ineq_sys ?g_sys v" for v
     using solves_ineq_sys_def by (metis length_g_sys)
 
-  have f_sol_of_g: "solves_eq_sys ?g_sys s \<longrightarrow> solves_eq_sys f_sys s" for s
+  have f_sol_of_g: "solves_eq_sys ?g_sys v \<longrightarrow> solves_eq_sys f_sys v" for v
     using solves_f_if_solves_g_eq solves_eq_sys_def
     by (metis add_0 diff_zero length_g_sys nth_map_upt)
 
